src/named/Core.v
@@ -1,1464 +1,201 @@
-Require Import mathcomp.ssreflect.all_ssreflect.
 Set Implicit Arguments.
-Unset Strict Implicit.
-Unset Printing Implicit Defensive.
 Set Bullet Behavior "Strict Subproofs".
 
+Require Import List String.
+Import ListNotations.
+Open Scope string.
+Open Scope list.
 From Utils Require Import Utils.
-From Named Require Import Exp Rule.
+From Named Require Import Exp ARule.
+
+(*TODO: why does this generate warnings?*)
 Import Exp.Notations.
-Import Rule.Notations.
-Require Import String.
+Import ARule.Notations.
 
-(* I want zip to be structural on s
-Definition zip' := 
-fun S T : Type =>
-fix zip (s : seq S) (t : seq T) {struct s} : seq (S * T) :=
-  match s with
-  | [::] => [::]
-  | x :: s' => match t with
-               | [::] => [::]
-               | y :: t' => (x, y) :: zip s' t'
-               end
-  end.
+Module Notations.
+  Export Exp.Notations.
+  Export ARule.Notations.
+End Notations.
 
-Lemma zip_zip' {S T} (s : seq S) (t : seq T) : zip s t = zip' s t.
-Proof using .
-  generalize t; clear t.
-  induction s; intro t; destruct t; simpl; f_equal; auto.
-Qed.
+Create HintDb lang_core discriminated.
 
- TODO: which version?
-Definition with_names_from (c : ctx) (l : list exp) : subst :=
-  (map (fun p => (fst (fst p), snd p)) (zip' c l)).
+Section TermsAndRules.
+  Context (l : lang).
 
-Lemma with_names_from_cons c l n t e
-  : with_names_from ((n,t)::c) (e::l)
-    = (n,e)::(with_names_from c l).
-Proof using .
-  cbn; f_equal.
-Qed.
-
-Lemma with_names_from_nil l : with_names_from [::] l = [::].
-Proof using.
-  cbn; f_equal.
-Qed.*)
-
-
-(* We could embed well-scopedness in bool, but well-typedness can be undecideable,
-   so we leave it in Prop.
-   Expression constructors contain the name of the sort/term rule that proves them wf.
-   
-   For all judgments except wf_ctx and wf_lang,
-   we assume the language and input context (where applicable) are well-formed.
-
-   For wf_args and wf_subst, we additionally assume the output context is well-formed.
-
-   For the relational judgments, we assume all arguments are well-formed.
-   The relational judgments accept the items to be related last to play well
-   with tactics.
- *)
-Inductive le_sort (l : lang) c : sort -> sort -> Prop :=
-| le_sort_by : forall name t1 t2,
-    [s> !c |- (name) {t1} = {t2}]%rule \in l ->
-    le_sort l c t1 t2
-| le_sort_subst : forall s1 s2 c' t1' t2',
-    le_subst l c c' s1 s2 ->
-    le_sort l c' t1' t2' ->
-    le_sort l c t1'[/s1/] t2'[/s2/]
-| le_sort_refl : forall t,
-    le_sort l c t t
-| le_sort_trans : forall t1 t12 t2,
-    le_sort l c t1 t12 ->
-    le_sort l c t12 t2 ->
-    le_sort l c t1 t2
-| le_sort_sym : forall t1 t2, le_sort l c t1 t2 -> le_sort l c t2 t1
-with le_term (l : lang) c : sort -> exp -> exp -> Prop :=
-| le_term_subst : forall s1 s2 c' t e1 e2,
-    le_subst l c c' s1 s2 ->
-    le_term l c' t e1 e2 ->
-    le_term l c t[/s2/] e1[/s1/] e2[/s2/]
-| le_term_by : forall name t e1 e2,
-    [:> !c |- (name) {e1} = {e2} : {t}]%rule \in l ->
-    le_term l c t e1 e2
-| le_term_refl : forall t e,
-    le_term l c t e e
-| le_term_trans : forall t e1 e12 e2,
-    le_term l c t e1 e12 ->
-    le_term l c t e12 e2 ->
-    le_term l c t e1 e2
-| le_term_sym : forall t e1 e2, le_term l c t e1 e2 -> le_term l c t e2 e1
-(* Conversion:
+  (*All assume wf_lang.
+    All ctxs (other than in wf_ctx) are assumed to satisfy wf_ctx.
+    Judgments whose assumptions take ctxs must ensure they are wf.
+    Sorts are not assumed to be wf; the term judgments should guarantee
+    that their sorts are wf.
+   *)
+  
+  Inductive le_sort : ctx -> sort -> sort -> Prop :=
+  | le_sort_by : forall c name t1 t2,
+      In (name, sort_le c t1 t2) l ->
+      le_sort c t1 t2
+  | le_sort_subst : forall c s1 s2 c' t1' t2',
+      (* Need to assert wf_ctx c here to satisfy
+         assumptions' presuppositions
+       *)
+      wf_ctx c' ->
+      le_subst c c' s1 s2 ->
+      le_sort c' t1' t2' ->
+      le_sort c t1'[/s1/] t2'[/s2/]
+  | le_sort_con : forall c name c' args s1 s2 es1 es2,
+      In (name, (sort_rule c' args)) l ->
+      le_args c c' s1 s2 args es1 es2 ->
+      le_sort c (scon name s1) (scon name s2)
+  | le_sort_trans : forall c t1 t12 t2,
+      le_sort c t1 t12 ->
+      le_sort c t12 t2 ->
+      le_sort c t1 t2
+  | le_sort_sym : forall c t1 t2, le_sort c t1 t2 -> le_sort c t2 t1
+  with le_term : ctx -> sort -> exp -> exp -> Prop :=
+  | le_term_subst : forall c s1 s2 c' t e1 e2,
+      (* Need to assert wf_ctx c' here to satisfy
+         assumptions' presuppositions
+       *)
+      wf_ctx c' ->
+      le_subst c c' s1 s2 ->
+      le_term c' t e1 e2 ->
+      le_term c t[/s2/] e1[/s1/] e2[/s2/]
+  | le_term_by : forall c name t e1 e2,
+      In (name,term_le c e1 e2 t) l ->
+      le_term c t e1 e2
+  | le_term_con : forall c name c' args t s1 s2 es1 es2,
+      In (name, (term_rule c' args t)) l ->
+      le_args c c' s1 s2 args es1 es2 ->
+      le_term c t[/with_names_from c' es2/] (con name s1) (con name s2)
+  | le_term_var : forall c x t,
+      In (x,t) c ->
+      le_term c t (var x) (var x)
+  | le_term_trans : forall c t e1 e12 e2,
+      le_term c t e1 e12 ->
+      le_term c t e12 e2 ->
+      le_term c t e1 e2
+  | le_term_sym : forall c t e1 e2, le_term c t e1 e2 -> le_term c t e2 e1
+  (* Conversion:
 
 c |- e1 = e2 : t 
                ||
 c |- e1 = e2 : t'
-*)
-| le_term_conv : forall t t',
-    le_sort l c t t' ->
-    forall e1 e2,
-    le_term l c t e1 e2 ->
-    le_term l c t' e1 e2
-with le_subst (l : lang) c : ctx -> subst -> subst -> Prop :=
-| le_subst_nil : le_subst l c [::] [::] [::]
-| le_subst_cons : forall c' s1 s2,
-    le_subst l c c' s1 s2 ->
-    forall name t e1 e2,
+   *)
+  | le_term_conv : forall c t t',
+      le_sort c t t' ->
+      forall e1 e2,
+        le_term c t e1 e2 ->
+        le_term c t' e1 e2
+  (* TODO: do I want to allow implicit elements in substitutions? *)
+  (* TODO: do I want to define this in terms of le_args? *)
+  with le_subst : ctx -> ctx -> subst -> subst -> Prop :=
+  | le_subst_nil : forall c, le_subst c [] [] []
+  | le_subst_cons : forall c c' s1 s2,
+      le_subst c c' s1 s2 ->
+      forall name t e1 e2,
+        (* assumed because the output ctx is wf: fresh name c' ->*)
+        le_term c t[/s2/] e1 e2 ->
+        le_subst c ((name, t)::c') ((name,e1)::s1) ((name,e2)::s2)
+  with le_args : ctx -> ctx -> list exp -> list exp -> list string -> list exp -> list exp -> Prop :=
+  | le_args_nil : forall c, le_args c [] [] [] [] [] []
+  | le_args_cons_ex : forall c c' s1 s2 args es1 es2,
+      le_args c c' s1 s2 args es1 es2 ->
+      forall name t e1 e2,
+        (* assumed because the output ctx is wf: fresh name c' ->*)
+        le_term c t[/with_names_from c' es2/] e1 e2 ->
+        le_args c ((name, t)::c') (e1::s1) (e2::s2) (name::args) (e1::es1) (e2::es2)
+  | le_args_cons_im : forall c c' s1 s2 args es1 es2,
+      le_args c c' s1 s2 args es1 es2 ->
+      forall name t e1 e2,
+        (* assumed because the output ctx is wf: fresh name c' ->*)
+        le_term c t[/with_names_from c' es2/] e1 e2 ->
+        le_args c ((name, t)::c') s1 s2 args (e1::es1) (e2::es2)
+  with wf_term : ctx -> exp -> sort -> Prop :=
+  | wf_term_by : forall c n s args c' t,
+      In (n, term_rule c' args t) l ->
+      wf_args c s c' ->
+      wf_term c (con n s) t[/(with_names_from c' s)/]
+  | wf_term_conv : forall c e t t',
+      (* We add this condition so that we satisfy the assumptions of le_sort
+         TODO: necessary? not based on current judgment scheme.
+         wf_term c e t should imply wf_sort c t,
+         and le_sort c t t' should imply wf_sort c t
+
+
+      wf_sort c t -> 
+       *)
+      wf_term c e t ->
+      le_sort c t t' ->
+      wf_term c e t'
+  | wf_term_var : forall c n t,
+      In (n, t) c ->
+      wf_term c (var n) t
+  with wf_args : ctx -> list exp -> ctx -> Prop :=
+  | wf_args_nil : forall c, wf_args c [] []
+  | wf_args_cons : forall c s c' name e t,
+      wf_term c e t[/with_names_from c' s/] ->
+      (* these arguments are last so that proof search unifies existentials
+       from the other arguments first*)
+      wf_args c s c' ->
+      wf_args c (e::s) ((name,t)::c')
+  with wf_sort : ctx -> sort -> Prop :=
+  | wf_sort_by : forall c n s args c',
+      In (n, (sort_rule c' args)) l ->
+      wf_args c s c' ->
+      wf_sort c (scon n s)
+  with wf_ctx : ctx -> Prop :=
+  | wf_ctx_nil : wf_ctx []
+  | wf_ctx_cons : forall name c v,
+      fresh name c ->
+      wf_ctx c ->
+      wf_sort c v ->
+      wf_ctx ((name,v)::c).
+  
+  Inductive wf_subst c : subst -> ctx -> Prop :=
+  | wf_subst_nil : wf_subst c [] []
+  | wf_subst_cons : forall s c' name e t,
       (* assumed because the output ctx is wf: fresh name c' ->*)
-      le_term l c t[/s2/] e1 e2 ->
-    le_subst l c ((name, t)::c') ((name,e1)::s1) ((name,e2)::s2).
+      wf_subst c s c' ->
+      wf_term c e t[/s/] ->
+      wf_subst c ((name,e)::s) ((name,t)::c').
 
-Inductive le_args (l : lang) c : ctx -> list exp -> list exp -> Prop :=
-| le_args_nil : le_args l c [::] [::] [::]
-| le_args_cons : forall c' s1 s2,
-    le_args l c c' s1 s2 ->
-    forall name t e1 e2,
-      (* assumed because the output ctx is wf: fresh name c' ->*)
-      le_term l c t[/with_names_from c' s2/] e1 e2 ->
-      le_args l c ((name, t)::c') (e1::s1) (e2::s2).
-
-
-Inductive wf_term l c : exp -> sort -> Prop :=
-| wf_term_by : forall n s c' t,
-    [:| !c' |- n : {t}]%rule \in l ->
-    wf_args l c s c' ->
-    wf_term l c (con n s) t[/(with_names_from c' s)/]
-| wf_term_conv : forall e t t',
-    (* We add this condition so that we satisfy the assumptions of le_sort *)
-    wf_sort l c t -> 
-    wf_term l c e t ->
-    le_sort l c t t' ->
-    wf_term l c e t'
-| wf_term_var : forall n t,
-    (n, t) \in c ->
-    wf_term l c (var n) t
-with wf_args l c : list exp -> ctx -> Prop :=
-| wf_args_nil : wf_args l c [::] [::]
-| wf_args_cons : forall (s : list exp) c' name e t,
-    (* assumed because the output ctx is wf: fresh name c' ->*)
-    wf_args l c s c' ->
-    wf_term l c e t[/with_names_from c' s/] ->
-    wf_args l c (e::s) ((name,t)::c')
-with wf_sort l c : sort -> Prop :=
-| wf_sort_by : forall n s c',
-    (n, (sort_rule c')) \in l ->
-    wf_args l c s c' ->
-    wf_sort l c (scon n s).
-
-Inductive wf_subst l c : subst -> ctx -> Prop :=
-| wf_subst_nil : wf_subst l c [::] [::]
-| wf_subst_cons : forall s c' name e t,
-    (* assumed because the output ctx is wf: fresh name c' ->*)
-    wf_subst l c s c' ->
-    wf_term l c e t[/s/] ->
-    wf_subst l c ((name,e)::s) ((name,t)::c').
-
-Inductive wf_ctx l : ctx -> Prop :=
-| wf_ctx_nil : wf_ctx l [::]
-| wf_ctx_cons : forall name c v,
-    fresh name c ->
-    wf_ctx l c ->
-    wf_sort l c v ->
-    wf_ctx l ((name,v)::c).
-
-
-Variant wf_rule l : rule -> Prop :=
-| wf_sort_rule : forall c,
-    wf_ctx l c ->
-    wf_rule l (sort_rule c)
-| wf_term_rule : forall c t,
-    wf_ctx l c ->
-    wf_sort l c t ->
-    wf_rule l (term_rule c t)
-| le_sort_rule : forall c t1 t2,
-    wf_ctx l c ->
-    wf_sort l c t1 ->
-    wf_sort l c t2 ->
-    wf_rule l (sort_le c t1 t2)
-| le_term_rule : forall c e1 e2 t,
-    wf_ctx l c ->
-    wf_sort l c t ->
-    wf_term l c e1 t ->
-    wf_term l c e2 t ->
-    wf_rule l (term_le c e1 e2 t).
-
-Inductive wf_lang : lang -> Prop :=
-| wf_lang_nil : wf_lang [::]
-| wf_lang_cons : forall l n r,
-    fresh n l ->
-    wf_lang l ->
-    wf_rule l r ->
-    wf_lang ((n,r)::l).
-
-(* build a database of presuppositions and judgment facts *)
-Create HintDb judgment discriminated.
-Hint Constructors wf_sort le_sort
-     wf_term le_term
-     wf_subst le_subst
-     wf_args le_args
-     wf_ctx wf_rule wf_lang : judgment.
+  Variant wf_rule : rule -> Prop :=
+  | wf_sort_rule : forall c args,
+      wf_ctx c ->
+      sublist args (map fst c) ->
+      wf_rule (sort_rule c args)
+  | wf_term_rule : forall c args t,
+      wf_ctx c ->
+      wf_sort c t ->
+      sublist args (map fst c) ->
+      wf_rule (term_rule c args t)
+  | le_sort_rule : forall c t1 t2,
+      wf_ctx c ->
+      wf_sort c t1 ->
+      wf_sort c t2 ->
+      wf_rule (sort_le c t1 t2)
+  | le_term_rule : forall c e1 e2 t,
+      wf_ctx c ->
+      wf_sort c t ->
+      wf_term c e1 t ->
+      wf_term c e2 t ->
+      wf_rule (term_le c e1 e2 t).
+  
+End TermsAndRules.
+  
+Hint Constructors le_sort le_term le_subst le_args
+     wf_sort wf_term wf_subst wf_args wf_ctx
+     wf_rule : lang_core.
 
 Scheme le_sort_ind' := Minimality for le_sort Sort Prop
+  with le_term_ind' := Minimality for le_term Sort Prop
   with le_subst_ind' := Minimality for le_subst Sort Prop
-  with le_term_ind' := Minimality for le_term Sort Prop.
-
-Combined Scheme le_ind
-         from le_sort_ind', le_subst_ind', le_term_ind'.
-
-Scheme wf_term_ind' := Minimality for wf_term Sort Prop
+  with wf_sort_ind' := Minimality for wf_sort Sort Prop
+  with wf_term_ind' := Minimality for wf_term Sort Prop
   with wf_args_ind' := Minimality for wf_args Sort Prop
-  with wf_sort_ind' := Minimality for wf_sort Sort Prop.
-
-Combined Scheme wf_ind
-         from wf_term_ind',
-         wf_args_ind',
-         wf_sort_ind'.
-
-Local Lemma wf_is_ws l c
-  : (forall e t, wf_term l c e t -> well_scoped (map fst c) e)
-    /\ (forall s c', wf_args l c s c' -> well_scoped (map fst c) s)
-    /\ (forall t, wf_sort l c t -> well_scoped (map fst c) t).
-Proof using .
-  apply wf_ind; intros; simpl in *; break_goal; auto.
-  eapply pair_fst_in; eauto.
-Qed.    
-
-Definition wf_term_ws l c := proj1 (wf_is_ws l c).
-Hint Resolve wf_term_ws : judgment.
-Definition wf_args_ws l c := proj1 (proj2 (wf_is_ws l c)).
-Hint Resolve wf_args_ws : judgment.
-Definition wf_sort_ws l c := proj2 (proj2 (wf_is_ws l c)).
-Hint Resolve wf_sort_ws : judgment.
-
-
-Lemma wf_is_ws_ctx l c : wf_ctx l c -> ws_ctx c.
-Proof using .
-  elim: c; simpl; first by auto.
-  intro_to wf_ctx; inversion; apply /andP; split; [apply /andP|]; eauto with judgment.
-Qed.
-Hint Resolve wf_is_ws_ctx : judgment.
-
-
-Definition get_rule_ctx (r : rule) : ctx :=
-  match r with
-  | sort_rule c => c
-  | term_rule c _ => c
-  | sort_le c _ _ => c
-  | term_le c _ _ _ => c
-  end.
-
-
-Definition get_rule_sort (r : rule) : sort :=
-  match r with
-  | sort_rule _ => {{s #"ERR"}}
-  | term_rule _ t => t
-  | sort_le _ _ _ => {{s #"ERR"}}
-  | term_le _ _ _ t => t
-  end.
-
-Lemma wf_sort_by' n l c : forall s,
-    let r := named_list_lookup (sort_rule [::]) l n in
-    let c' := get_rule_ctx r in
-    (n, (sort_rule c')) \in l ->
-    wf_args l c s c' ->
-    wf_sort l c (scon n s).
-Proof using .
-  intros.
-  econstructor; eassumption.
-Qed.
-
-Lemma wf_term_by' n l c : forall s t,
-    let r := named_list_lookup (sort_rule [::]) l n in
-    let c' := get_rule_ctx r in
-    let t' := get_rule_sort r in
-    (n, (term_rule c' t')) \in l ->
-    wf_args l c s c' ->   
-    t = t'[/with_names_from c' s/] ->
-    wf_term l c (con n s) t.
-Proof using .
-  intros.
-  rewrite H1.
-  eapply wf_term_by; eassumption.
-Qed.
-
-
-Lemma wf_term_var' n l c t :
-    (n, t) \in c ->
-    wf_term l c (var n) t.
-Proof using .
-  constructor; assumption.
-Qed.
-
-
-Lemma wf_subst_len_eq l c s c' : wf_subst l c s c' -> size s = size c'.
-Proof using .
-  elim: s c'.
-  - case; simpl; auto; intro_to wf_subst; by inversion.
-  - intros until c'; elim: c'.
-    + simpl; auto; intro_to wf_subst; by inversion.
-    + simpl; intros; f_equal;
-      specialize H with l1; destruct H;
-      inversion H1;
-      eauto with judgment.
-Qed.
-Hint Resolve wf_subst_len_eq : judgment.
-
-
-Lemma wf_args_len_eq l c s c' : wf_args l c s c' -> size s = size c'.
-Proof using .
-  elim: s c'.
-  - case; simpl; auto; intro_to wf_args; by inversion.
-  - intros until c'; elim: c'.
-    + simpl; auto; intro_to wf_args; by inversion.
-    + simpl; intros; f_equal;
-      specialize H with l1; destruct H;
-      inversion H1;
-      eauto with judgment.
-Qed.
-Hint Resolve wf_args_len_eq : judgment.
-
-
-Lemma le_subst_len_eq_r l c c' s1 s2 : le_subst l c c' s1 s2 -> size s2 = size c'.
-Proof using .
-  elim: s2 s1 c'.
-  - case; intros until c'; case:c'; simpl; auto; intro_to le_subst; by inversion.
-  - intros until s1; case:s1; intros until c'; case:c';
-      try by (intro_to le_subst; inversion).
-    simpl; intros; f_equal.
-    inversion H0; eauto.
-Qed.
-Hint Resolve le_subst_len_eq_r : judgment.
-
-Lemma le_subst_len_eq_l l c c' s1 s2 : le_subst l c c' s1 s2 -> size s1 = size c'.
-Proof using .
-  elim: s1 s2 c'.
-  - case; intros until c'; case:c'; simpl; auto; intro_to le_subst; by inversion.
-  - intros until s2; case:s2; intros until c'; case:c';
-      try by (intro_to le_subst; inversion).
-    simpl; intros; f_equal.
-    inversion H0; eauto.
-Qed.
-Hint Resolve le_subst_len_eq_l : judgment.
-
-
-
-(* TODO
-Lemma wf_is_ws_rule l r : wf_rule l r -> ws_rule r.
-Proof.
-  case: r; intro_to wf_rule; inversion; simpl.
-  all: try repeat (apply /andP; split).
-  all:eauto with judgment.
-  give_up(*TODO: prob have to show directly *).
-Admitted.
-Hint Resolve wf_is_ws_rule : judgment.
-*)
-
-Lemma le_subst_refl l c s c' : wf_subst l c s c' -> le_subst l c c' s s.
-Proof using .
-  elim; econstructor; eauto with judgment.
-Qed.
-Hint Resolve le_subst_refl : judgment.
-
-Lemma wf_subst_names_eq l c s c'
-  : wf_subst l c s c' -> map fst s = map fst c'.
-Proof using .
-  elim; intros; simpl in *; eauto.
-  f_equal; auto.
-Qed.
-Hint Resolve wf_subst_names_eq : judgment.
-
-Lemma le_subst_names_eq_l l c c' s1 s2
-  : le_subst l c c' s1 s2 -> map fst s1 = map fst c'.
-Proof using .
-  elim; intros; simpl in *; eauto.
-  f_equal; auto.
-Qed.
-Hint Resolve le_subst_names_eq_l : judgment.
-
-
-Lemma le_subst_names_eq_r l c c' s1 s2
-  : le_subst l c c' s1 s2 -> map fst s2 = map fst c'.
-Proof using .
-  elim; intros; simpl in *; eauto.
-  f_equal; auto.
-Qed.
-Hint Resolve le_subst_names_eq_r : judgment.
-
-(* TODO: get proofs through*)
-
-(* Monotonicity under substitution
-TODO: need wf_ctx for c' is subst case? (to get ws) *)
-Lemma mono_le_subst l c
-  : (forall t1 t2,
-        le_sort l c t1 t2 ->
-        forall c' s1 s2, le_subst l c' c s1 s2 ->
-                         le_sort l c' t1[/s1/] t2[/s2/])
-    /\ (forall c' s1 s2,
-           le_subst l c c' s1 s2 -> ws_ctx c' ->
-           forall c'' s1' s2', le_subst l c'' c s1' s2' ->
-                               le_subst l c'' c' s1[/s1'/] s2[/s2'/])
-    /\ (forall t e1 e2,
-           le_term l c t e1 e2 -> well_scoped (map fst c) t ->
-           forall c' s1 s2, le_subst l c' c s1 s2 ->
-                            le_term l c' t[/s2/] e1[/s1/] e2[/s2/]).
-Proof with eauto with judgment using.
-  move: c; apply: le_ind; intros; break; simpl in *; break...
-  constructor; fold_Substable...
-  rewrite <-subst_assoc...
-  erewrite le_subst_names_eq_r...
-Qed.
-
-Definition le_subst_sort l c := proj1 (mono_le_subst l c).
-Hint Resolve le_subst_sort : judgment.
-Definition le_subst_subst l c := proj1 (proj2 (mono_le_subst l c)).
-Hint Resolve le_subst_subst : judgment.
-Definition le_subst_term l c := proj2 (proj2 (mono_le_subst l c)).
-Hint Resolve le_subst_term : judgment.
-
-Lemma map_fst_with_names_from (c:ctx) (s : list exp)
-  : size s = size c -> map fst (with_names_from c s) = map fst c.
-Proof using .
-  elim: c s; intros until s; case: s; intros; break;simpl in *; auto.
-  { inversion H0. }
-  {
-    f_equal; auto.
-  }
-Qed.
-
-Lemma map_snd_with_names_from  (c:ctx) (s : list exp)
-  : size s = size c -> map snd (with_names_from c s) = s.
-Proof using .
-  elim: c s; intros until s; case: s; intros; break;simpl in *; auto.
-  { inversion H. }
-  {
-    f_equal; auto.
-  }
-Qed.
-
-Lemma wf_subst_lookup l c s c' n t
-  : wf_subst l c s c' -> wf_ctx l c' -> (n,t) \in c' ->  wf_term l c (subst_lookup s n) t [/s /].
-Proof using .
-  elim; intros; simpl in *; [ easy|].
-  inversion H2; subst; clear H2.
-  move: H3.
-  rewrite in_cons.
-  change ((?a,?b)==(?c,?d)) with ((a==c)&&(b==d)).
-  change (n =? name)%string with (n == name).
-  case neq: (n== name); simpl.
-  case teq: (t==t0); simpl.
-  {
-    move: neq teq => /eqP neq /eqP teq _.
-    subst.
-    rewrite ws_sort_mono; auto.
-    simpl in *.
-    all: erewrite wf_subst_names_eq; eauto with judgment.
-  }
-  {
-    move: neq => /eqP neq; subst.
-    intros; exfalso.
-    suff: (name != name).
-    { rewrite eq_refl; done. }
-    eapply fresh_neq_in_fst; eauto using pair_fst_in.
-  }
-  {
-    intro.
-    rewrite ws_sort_mono; auto.
-    {
-      simpl in *.
-      erewrite wf_subst_names_eq; eauto with judgment.
-    }
-    {
-      erewrite wf_subst_names_eq; eauto.
-      eapply sort_in_ws; eauto with judgment.
-    }
-  }
-Qed.      
-  
-Lemma mono_wf_subst l c
-  : ws_lang l (*TODO: just used for wsness; handle differently? ws syntax?*)->
-    (forall e t,
-           wf_term l c e t ->
-           wf_ctx l c ->
-           well_scoped (map fst c) t ->
-           forall c' s, wf_subst l c' s c ->
-                        wf_term l c' e[/s/] t[/s/])
-    /\ (forall s c',
-           wf_args l c s c' ->
-           wf_ctx l c ->
-           ws_ctx c' ->
-           forall c'' s', wf_subst l c'' s' c ->
-                          wf_args l c'' s[/s'/] c')
-    /\ (forall t,
-           wf_sort l c t -> wf_ctx l c ->
-           forall c' s, wf_subst l c' s c ->
-                        wf_sort l c' t[/s/]).
-Proof with eauto with judgment using .
-  move => wsl; apply wf_ind; intros; simpl in *; break_andbs...
-  {
-    rewrite subst_assoc.
-    {
-      fold_Substable.
-      rewrite -with_names_from_args_subst.
-      apply wf_term_by...
-      apply H1...
-      apply rule_in_ws in H...
-      simpl in H.
-      by break.
-    }
-    {
-      rewrite map_fst_with_names_from...
-      apply rule_in_ws in H...
-      simpl in H; by break.
-    }
-  }
-  {
-    eapply wf_term_conv.
-    apply H0...
-    apply H2...
-    eapply le_subst_sort...
-  }
-  {
-    eauto using wf_subst_lookup.
-  }
-  {
-    econstructor...
-    rewrite with_names_from_args_subst.
-    rewrite -subst_assoc ?map_fst_with_names_from...
-    {
-      apply H2...
-      change (sort_subst ?s ?t) with t[/s/].
-      apply ws_sort_subst.
-      {
-        rewrite ws_subst_args.
-        break_goal; simpl; rewrite ?map_snd_with_names_from ?map_fst_with_names_from...
-        apply ws_all_fresh_ctx...
-      }
-      {
-        rewrite map_fst_with_names_from...
-      }
-    }
-  }
-  {
-    econstructor; eauto.
-    apply H1; eauto.
-    apply rule_in_ws in H; auto.
-  }
-Qed.
-
-Definition wf_subst_term l c wfl := proj1 (@mono_wf_subst l c wfl).
-Hint Resolve wf_subst_term : judgment.
-
-Definition wf_args_subst l c wfl :=
-  proj1 (proj2 (@mono_wf_subst l c wfl)).
-Hint Resolve wf_args_subst : judgment.
-
-Definition wf_sort_subst l c wfl :=
-  proj2 (proj2 (@mono_wf_subst l c wfl)).
-Hint Resolve wf_sort_subst : judgment.
-
-
-Lemma mono_ext_le l n r c
-  : (forall t1 t2,
-        le_sort l c t1 t2 -> wf_rule l r ->
-        le_sort ((n,r)::l) c t1 t2)
-    /\ (forall s1 s2 c',
-           le_subst l c s1 s2 c' ->
-           wf_rule l r ->
-           le_subst ((n,r)::l) c s1 s2 c')
-    /\ (forall e1 e2 t,
-           le_term l c e1 e2 t ->
-           wf_rule l r ->
-           le_term ((n,r)::l) c e1 e2 t).
-Proof with eauto with judgment using.
-  move: c; apply le_ind...
-  all: intro_to is_true; intro H; constructor...
-  {
-    apply le_sort_sym.
-    eapply le_sort_by.
-    rewrite in_cons.
-    apply /orP; right.
-    eassumption.
-  }
-  {
-    apply le_term_sym.
-    eapply le_term_by.
-    rewrite in_cons.
-    apply /orP; right.
-    eassumption.
-  }
-Qed.
-
-Lemma mono_ext_wf l n r c  
-    : (forall e t,
-          wf_term l c e t -> wf_ctx l c -> wf_rule l r ->  wf_term ((n,r)::l) c e t)
-      /\ (forall s c',
-           wf_args l c s c' -> wf_ctx l c -> wf_rule l r -> wf_args ((n,r)::l) c s c')
-      /\ (forall t,
-           wf_sort l c t -> wf_ctx l c -> wf_rule l r -> wf_sort ((n,r)::l) c t).
-Proof with eauto with judgment using .
-  apply wf_ind...
-  all: try by econstructor; eauto with judgment; rewrite in_cons; apply /orP; auto.
-  {
-    econstructor...
-    eapply mono_ext_le...
-  }
-Qed.
-(* TODO: add as hint? *)
-
-Lemma mono_ext_ctx l n r c : wf_rule l r -> wf_ctx l c -> wf_ctx ((n,r)::l) c.
-Proof.
-  elim: c; simpl; intro_to wf_ctx; inversion; subst; constructor;
-    eauto with judgment.
-  eapply mono_ext_wf; eauto with judgment.  
-Qed.
-
-Lemma mono_ext_rule l n r r' : wf_rule l r -> wf_rule l r' -> wf_rule ((n,r)::l) r'.
-Proof using .
-  move => wfr.
-  inversion; constructor; try by constructor; auto.
-  all: try by eapply mono_ext_wf...
-  all: eapply mono_ext_ctx; eauto with judgment.
-Qed.
-
-(*
-Lemma wf_lang_prefix l1 l2 : wf_lang (l1 ++ l2) -> wf_lang l2.
-Proof using .
-  elim: l1; auto.
-  move => r l1 IH.
-  rewrite cat_cons => wfl.
-  inversion wfl.
-  eauto.
-Qed.
-
-Lemma wf_lang_rst : forall l a, wf_lang (a :: l) -> wf_lang l.
-Proof using .
-  intro_to wf_lang; inversion; eauto.
-Qed.
-*)
-
-Lemma rule_in_wf l r n : wf_lang l -> (n,r) \in l -> wf_rule l r.
-Proof using .
- elim; first by compute.
- intro_to wf_lang; intro_to is_true.
- rewrite in_cons; case /orP.
- {
-   move /eqP; case => _ ->.
-   eapply mono_ext_rule; auto.
- }
- {
-   move /H1.
-   eapply mono_ext_rule; auto.
- }   
-Qed.
-Hint Resolve rule_in_wf : judgment.
-
-Lemma le_subst_trans l c c' s1 s2 s3
-  : le_subst l c c' s1 s2 -> le_subst l c c' s2 s3 ->
-    le_subst l c c' s1 s3.
-Proof using .
-  elim: s1 s2 s3 c';
-    intros until s2; case: s2;
-    intros until s3; case: s3;
-    intros until c'; case: c';
-      eauto with judgment;
-      intro_to le_subst; repeat inversion; subst.
-  econstructor; eauto with judgment.
-Qed.
-
-(*
-Lemma exp_subst_strengthen e s2 e2
-  : ws_exp (size s2) e -> e[/e2::s2/] = e[/s2/].
-Proof.
-  elim: e.
-  {
-    intro n.
-    unfold exp_subst.
-    unfold var_lookup.
-    unfold nth_level.
-    simpl.
-    intro nlt.
-    suff: (n < (size s2).+1).
-    move => ->.
-    rewrite nlt.
-    (*TODO: some nat math*)
-Admitted.
-
-Lemma subst_cmp_strengthen e s2 s1
-  : ws_subst (size s2) s1 -> subst_cmp s1 (e::s2) = subst_cmp s1 s2.
-Proof.
-  elim s1; simpl; auto.
-  move => e1 s1' IH /andP [wse wss].
-  f_equal; eauto using exp_subst_strengthen.
-Qed.
-
-
-
-Lemma id_subst_cmp s : (subst_cmp (id_subst (size s)) s) = s.
-Proof.
-  remember (size s) as sz.
-  move: Heqsz.
-  elim: sz s; simpl.
-  {
-    intros s H; symmetry in H; move: H.
-    by move /size0nil.
-  }
-  {
-    intros n IH; case; simpl.
-    by move => /eqP //=.
-    intros e s; case.
-    intro neq.
-    rewrite id_subst_size.
-    f_equal.
-    {
-      unfold exp_subst; simpl.
-      rewrite neq.
-      unfold var_lookup.
-      unfold nth_level.
-      simpl.
-      rewrite ltnSn.
-      by rewrite sub_n_n.
-    }
-    {
-      rewrite subst_cmp_strengthen; eauto with judgment.
-      (*TODO: fairly easy*)
-      give_up.
-    }
-  }      
-Admitted.
-
-Lemma id_subst_le l c c'
-      : le_subst l c c' (id_subst (size c')) (id_subst (size c')).
-Proof.
-Admitted.
-Hint Resolve id_subst_le : judgment.
-
-Lemma le_mono_ctx l c
-  : (forall t1 t2,
-        le_sort l c t1 t2 ->
-        forall c', le_sort l (c' ++ c) t1 t2)
-    /\ (forall c' s1 s2,
-           le_subst l c c' s1 s2 ->
-           forall c'', le_subst l (c'' ++ c) c' s1 s2)
-    /\ (forall t e1 e2,
-           le_term l c t e1 e2 ->
-           forall c', le_term l (c' ++ c) t e1 e2).
-Proof with eauto with judgment using.
-  move: c; apply le_ind...
-  {
-    intros.
-    elim: c'; simpl...
-    intros e c' IH.
-    rewrite -(@id_subst_identity t1 (size(c'++c)))
-    -(@id_subst_identity t2 (size(c'++c))).
-    eapply le_sort_subst...
-  }
-  {
-    intros.
-    elim: c'; simpl...
-    intros e c' IH.
-    rewrite -(@id_subst_identity e1 (size(c'++c)))
-    -(@id_subst_identity e2 (size(c'++c)))
-    -(@id_subst_identity t (size(c'++c))).
-    eapply le_term_subst...
-  }
-Qed.
-
-
-Lemma wf_ctx_suffix l c' c : wf_ctx l (c' ++ c) -> wf_ctx l c.
-Proof using .
-  elim: c'; auto; simpl.
-  intro_to wf_ctx; inversion; eauto.
-Qed.
-Hint Resolve wf_ctx_suffix : judgment.
-
-
-Lemma wf_ctx_tail l t c : wf_ctx l (t :: c) -> wf_ctx l c.
-Proof using .
-  intro_to wf_ctx; inversion; eauto.
-Qed.
-Hint Resolve wf_ctx_tail : judgment.
-
-Lemma id_subst_wf l c c'
-      : wf_subst l (c'++ c) (id_subst (size c)) c.
-Proof.
-Admitted.
-Hint Resolve id_subst_wf : judgment.
-
-
-
-Lemma is_nth_level_suffix {A : eqType} c' c n (t : A) : is_nth_level c n t -> is_nth_level (c'++c) n t.
-Proof using .
-  elim: c'; simpl; auto using is_nth_level_cons.
-Qed.
-Hint Resolve is_nth_level_suffix : judgment.
-
-Lemma wf_mono_ctx l c
-  : wf_lang l ->
-    (forall t,
-        wf_sort l c t ->
-        forall c', wf_ctx l (c' ++ c) -> wf_sort l (c' ++ c) t)
-    /\ (forall s c',
-           wf_subst l c s c' ->
-           forall c'', wf_ctx l (c'' ++ c) ->
-                       wf_subst l (c'' ++ c) s c')
-    /\ (forall e t,
-           wf_term l c e t ->
-           forall c', wf_ctx l (c' ++ c) ->
-                      wf_term l (c' ++ c) e t).
-Proof with eauto with judgment using .
-  move => wfl.
-  move: c; apply wf_ind...
-  {
-    intros until c'.
-    elim: c'; simpl...
-    intros e' c' IH wfc.
-    rewrite -(@id_subst_identity e (size(c'++c)))
-    -(@id_subst_identity t' (size(c'++c))).
-    change (e'::(c'++c)) with ([::e']++(c'++c)).
-    eapply mono_subst_wf_term...
-  }
-Qed.
-
-*)
-Lemma subst_sym l c c' s1 s2 : le_subst l c c' s1 s2 -> le_subst l c c' s2 s1.
-Proof using.
-  elim; eauto with judgment.
-Qed.
-
-(* Preservation of judgments under rewriting *)
-Add Parametric Relation l c : sort (le_sort l c)
-    reflexivity proved by (le_sort_refl l c)
-    symmetry proved by (@le_sort_sym l c)
-    transitivity proved by (@le_sort_trans l c)
-      as le_sort_rel.
-Add Parametric Relation l c c' : subst (le_subst l c c')
-   (*reflexivity proved by (le_subst_refl l c)
-     not reflexive unless I implement ws syntax
-    *)
-    symmetry proved by (@subst_sym l c c')
-    transitivity proved by (@le_subst_trans l c c')
-   as le_subst_rel.
-Add Parametric Relation l c t : exp (le_term l c t)
-    reflexivity proved by (le_term_refl l c t)
-    symmetry proved by (@le_term_sym l c t)
-    transitivity proved by (@le_term_trans l c t)
-   as le_term_rel.
-
-Require Import Setoid Morphisms Program.Basics.
-
-Add Parametric Morphism l c c' : sort_subst
-  with signature le_subst l c c' ==> (le_sort l c') ==>(le_sort l c) as sort_subst_mor.
-Proof using .
-  intro_to le_sort; inversion;
-    eauto with judgment.
-Qed.
-
-Definition dep_respectful {A : Type} {B : Type}
-           (R : relation A) (R' : A -> A -> relation B) :=
-    Eval compute in @respectful_hetero A A (fun _ => B) (fun _ => B) R R'.
-Local Notation "@( x , y ) : R , R'" :=
-  (@dep_respectful _ _ (R%signature) (fun x y =>R'%signature))
-    (right associativity, at level 56) : signature_scope.
-
-(* We have to write the instance manually because dep_respectful
-   isn't yet supported by the automatic machinery*)
-Instance term_subst_mor_Proper (l : lang) (c c': ctx) t
-  : Morphisms.Proper (@(_,s2) : (le_subst l c c'), le_term l c' t ==> le_term l c t[/s2/])%signature exp_subst.
-Proof using .
-  unfold Proper.
-  unfold dep_respectful.
-  unfold respectful.
-  eauto with judgment.
-Qed.
-
-Definition term_subst_mor  : forall (l : lang) (c c' : ctx) (t : sort) (x y : subst),
-       le_subst l c c' x y ->
-       forall x0 y0 : exp, le_term l c' t x0 y0 -> le_term l c t[/y/] x0 [/x /] y0 [/y /].
-  refine (fun (l : lang) (c c' : ctx) (t : sort) => _).
-  eapply @proper_prf.
-  eauto with typeclass_instances.
-  Unshelve.
-  eapply term_subst_mor_Proper.
-Defined.
-
-(* TODO
-Add Parametric Morphism l c c' c'' (_:ws_ctx c'') : subst_cmp
-    with signature le_subst l c' c'' ==> le_subst l c c' ==> le_subst l c c''
-      as subst_subst_mor.
-Proof with eauto with judgment using.
-  intro_to le_subst; intros les; elim: les H...
-Qed.
- *)
-
-(*
-Add Parametric Morphism l c c' n : (srt n)
-    with signature le_args l c c' ==> le_sort l c as sort_con_mor.
-Proof using .
-(*  intros.
-  suff: (le_sort l c (con n (id_subst (size c')))[/x/] (con n (id_subst (size c')))[/y/]);
-    eauto with judgment.
-  rewrite !con_subst_cmp.
-  erewrite <-le_subst_len_eq_l at 1; eauto.
-  replace (size c') with (size y).
-  rewrite !id_subst_cmp.
-  eauto with judgment.
-  erewrite le_subst_len_eq_r; eauto.
-Qed.*)
-Admitted.
-
-(* We have to write the instance manually because dep_respectful
-   isn't yet supported by the automatic machinery*)
-Instance args_cons_mor_Proper (l : lang) (c c': ctx) t name
-  : Morphisms.Proper (@(_,s2) : (le_args l c c'), le_term l c t[/with_names_from c' s2/] ==> le_args l c ((name,t)::c'))%signature
-                     (flip cons).
-Proof using .
-  unfold Proper.
-  unfold dep_respectful.
-  unfold respectful.
-  unfold flip.
-  eauto with judgment.
-Admitted.
-
-Definition args_cons_mor  : forall (l : lang) (c c' : ctx) (t : sort) name (x y : list exp),
-       le_args l c c' x y ->
-       forall x0 y0 : exp, le_term l c t[/with_names_from c' y/] x0 y0 -> le_args l c ((name,t)::c') (x0::x) (y0::y).
-  refine (fun (l : lang) (c c' : ctx) (t : sort) name => _).
-  eapply @proper_prf.
-  eauto with typeclass_instances.
-  Unshelve.
-  apply args_cons_mor_Proper.
-Defined.
-*)
-
-(* TODO
-Instance term_con_mor_Proper (l : lang) (c c': ctx) n t
-  : Morphisms.Proper (@(_,s2) : (le_subst l c c'), le_term l c t[/s2/])%signature (con n).
-Proof using .
-  unfold Proper.
-  unfold dep_respectful.
-  intros.
-  suff: (le_term l c t[/y/] (con n (id_subst (size c')))[/x/] (con n (id_subst (size c')))[/y/]);
-    eauto with judgment.
-  rewrite !con_subst_cmp.
-  erewrite <-le_subst_len_eq_l at 1; eauto.
-  replace (size c') with (size y).
-  rewrite !id_subst_cmp.
-  eauto with judgment.
-  erewrite le_subst_len_eq_r; eauto.
-Qed.
-
-Definition term_con_mor  : forall (l : lang) (c c' : ctx) n (t : exp) (x y : subst),
-       le_subst l c c' x y -> le_term l c t[/y/] (con n x) (con n y).
-  refine (fun (l : lang) (c c' : ctx) n (t : exp) => _).
-  eapply @proper_prf.
-  eauto with typeclass_instances.
-  Unshelve.
-  eapply term_con_mor_Proper.
-Defined.
-*)
-
-
-(*TODO: should this be true?/do I need it to be true?
-Lemma wf_term_subst_mor l c (_:wf_lang l)
-  : (forall s1 s2 c', le_subst l c s1 s2 c' -> wf_subst l c s1 c' <-> wf_subst l c s2 c')
-    /\ (forall e1 e2 t, le_term l c e1 e2 t -> wf_term l c e1 t <-> wf_term l c e2 t).
-Proof.
-  Scheme le_subst_ind'' := Minimality for le_subst Sort Prop
-    with le_term_ind'' := Minimality for le_term Sort Prop.
-  Combined Scheme le_ind' from le_subst_ind'', le_term_ind''.
-  move: c; apply: le_ind'; eauto with judgment.
-  by split; intro_to wf_subst; inversion; subst; constructor; eauto with judgment.
-  {
-    intros;
-      repeat match goal with H : _ <-> _ |- _ => destruct H end;
-      split; inversion; subst; constructor; eauto with judgment.
-    give_up (* TODO: this is sim. to issues past*)
-    by apply H1.
-    
-  give_up (*subst term case; hard*).
-  {
-    intro_to is_true.
-    move /(rule_in_wf H).
-    by inversion.
-  }
-  { (*Conv
-      Needs to be iff for this case?
-      TODOTODOTODOTODO: this case is very bad!
-      only hope? show that
-
-*)
- 
-  
-  intro_to wf_term; inversion; subst.
-              | constructor]; eauto with judgment.
-  {
-     subst.
-    constructor; eauto with judgment.
-      
-Add Parametric Morphism l c c' : (flip (wf_subst l c) c')
-    with signature subst_sig l c c' ==> impl as wf_subst_mor.
-Proof.
-  unfold impl.
-  intros s1 s2.
-  elim; eauto with judgment.
-  TODO: must be mutual w/ terms.
-  
-Add Parametric Morphism l c : (wf_sort l c)
-    with signature le_sort l c ==> impl as wf_sort_mor.
-Proof.
-Add Parametric Morphism l c : (wf_sort l c)
-    with signature le_sort l c ==> impl as wf_sort_mor.
-Proof.
-  unfold impl.
- *)
-(*
-
-(* TODO:put somewhere better?*)
-Lemma wf_ctx_in l c t : wf_lang l -> wf_ctx l c -> t \in c -> wf_sort l c t.
-Proof using .
-  intro wfl.
-  elim: c; simpl; intro_to is_true; try by compute.
-  rewrite in_cons.
-  inversion H0; subst.
-  move /orP; case.
-  move /eqP ->.
-  all: intros; change (a::l0) with ([::a]++l0);
-  do [eapply le_mono_ctx| eapply wf_mono_ctx];
-  eauto with judgment.
-Qed.
-
-Lemma wf_term_sort l c e t : wf_lang l -> wf_ctx l c -> wf_term l c e t -> wf_sort l c t.
-Proof using .
-  intros wfl wfc wft.
-  elim: wft wfc; intros; eauto with judgment.
-  {
-    move: H => /is_nth_level_in;
-    move /(rule_in_wf wfl);
-    inversion; eauto with judgment.  
-  }
-  {
-    move: H => /is_nth_level_in;
-                 auto using wf_ctx_in.
-  }
-Qed.
-Hint Immediate wf_term_sort : judgment.
-
-(*TODOTODOTODOTODOTODO: evaluate everything below this line *)
-(*
-
-Lemma is_nth_level_cat {A : eqType} l (a : A) l' : is_nth_level (l ++ a :: l') (size l') a.
-Proof using .
-  unfold is_nth_level.
-  apply /andP; split;
-  rewrite size_cat; simpl.
-  apply: ltn_addl; auto.
-  rewrite addnC; rewrite add_sub.
-  elim: l; simpl; auto.
-Qed.
-
-
-(* TODO: move to utils *)
-Ltac rewrite_matching lem c :=
-      match goal with [ H : context[c] |- _] =>
-                      rewrite lem in H end.
-
-
-Lemma subst_nil e : e [/[::]/] = e.
-Proof using .
-  elim: e; auto.
-  unfold exp_subst; intros; simpl.
-  f_equal.
-  elim: l H; simpl; auto.
-  intros.
-  f_equal; tauto.
-Qed.
-
-Lemma subst_strengthen s' s e : ws_exp (size s) e -> e[/s'++s/] = e[/s/].
-Proof using .
-  elim: e.
-  {
-    unfold exp_subst; simpl; intros.
-    unfold var_lookup.
-    unfold nth_level.
-    rewrite size_cat H.
-    suff: n < size s' + size s => [->|].
-    rewrite nth_cat.
-    rewrite -addnBA; auto.
-    rewrite -ltn_subRL.
-    rewrite sub_n_n; simpl.
-    by rewrite add_sub.
-    by apply ltn_addl.
-  }
-  {
-    intro n; elim; auto.
-    unfold exp_subst; simpl.
-    intro_to and; case.
-    intro_to is_true; case /andP.
-    intros; f_equal; f_equal; auto.
-    move: (H b b0); case; auto.
-  }
-Qed.
- 
-Lemma wf_subst_drop n l c' s c : wf_subst l c' s c -> wf_subst l c' (drop n s) (drop n c).
-Proof using .
-  elim: n s c; first intros; rewrite ?drop0; auto.
-  intros until s; case: s; intros until c; case: c; intro_to wf_subst; inversion; simpl; eauto with judgment.
-Qed.
-  
-Lemma wf_nth l c' s c a b n : n < size c -> wf_subst l c' s c -> wf_term l c' (nth a s n) (nth b c n) [/s/].
-Proof using .
-  intros.
-  erewrite <-(@cat_take_drop n _ s).
-  erewrite <-(@cat_take_drop n _ c).
-  rewrite !nth_cat.
-  suff: n < size s; [ intro nlts | erewrite wf_subst_len_eq; eauto].
-  rewrite !size_takel; auto.
-  rewrite !ltnn.
-  rewrite !sub_n_n !nth0.
-  move: H0 => /(@wf_subst_drop n).
-  generalize (take n s) as s'.
-  elim: n c s H nlts; intros until c; case: c; try easy; intros until s; case: s; try easy.
-  {
-    intros e s t c; simpl.
-    intro_to wf_subst; inversion; subst.
-    rewrite -cat_rcons.
-    rewrite subst_strengthen; auto.
-    erewrite wf_subst_len_eq; eauto with judgment.
-  }
-  {
-    intros.
-    simpl.
-    eauto with judgment.
-  }
-Qed.
-
-
-Lemma ws_exp_mono sz e : ws_exp sz e -> ws_exp sz.+1 e.
-Proof using .
-  elim: e; simpl; auto.
-  intros until l; elim: l; simpl; auto.
-  intro_to and; case.
-  intro_to is_true; move /andP; case.
-  intros; apply /andP; split.
-  exact (a0 a1).
-  apply: H; auto.
-Qed.
-  
-Lemma ws_ctx_nth l c a n : n < size c -> wf_ctx l c -> ws_exp (size c) (nth a c n).
-Proof using .
-  elim: n c; intros until c; case: c; try easy.
-  all: intro_to wf_ctx; inversion; simpl.
-  all: apply: ws_exp_mono; eauto with judgment.
-Qed.
-
-Lemma mono_n l'
-  :  (forall (l : lang) c t1 t2,
-        le_sort l c t1 t2 -> wf_lang (l' ++ l) ->
-        le_sort (l'++l) c t1 t2)
-    /\ (forall (l : lang) c s1 s2 c',
-           le_subst l c s1 s2 c' ->
-           wf_lang (l' ++ l) ->
-           le_subst (l'++l) c s1 s2 c')
-    /\ (forall (l : lang) c e1 e2 t,
-           le_term l c e1 e2 t ->
-           wf_lang (l' ++ l) ->
-           le_term (l'++l) c e1 e2 t)
-    /\ (forall (l : lang) c t,
-           wf_sort l c t -> wf_lang (l' ++ l) -> wf_sort (l'++l) c t)
-    /\ (forall (l : lang) c s c',
-           wf_subst l c s c' -> wf_lang (l' ++ l) -> wf_subst (l'++l) c s c')
-    /\ (forall (l : lang) c e t,
-           wf_term l c e t -> wf_lang (l' ++ l) -> wf_term (l'++l) c e t)
-    /\ (forall (l : lang) c,
-           wf_ctx l c -> wf_lang (l' ++ l) ->  wf_ctx (l'++l) c).
-Proof using .
-  elim: l'; simpl;
-    try by repeat match goal with |- _/\_ => split end;
-    intros; rewrite ?constr_shift0 ?map_constr_shift0.
-  intros.
-  repeat match goal with |- _/\_ => split end;
-    intros.
-  all: by eapply mono;
-  [eapply H; auto; inversion H1; apply: wf_rule_lang; eauto|
-    by inversion H1].
-Qed.
-
-   
-Scheme wf_rule_lang_ind := Induction for wf_rule Sort Prop
-  with wf_lang_lang_ind := Induction for wf_lang Sort Prop.
-
-
-
-Ltac suff_to_use H :=
-   match goal with
-    | |- ?T =>
-      let T' := type of H in
-      suff: T = T' => [-> //|]; f_equal
-   end.
-
-
-Lemma add_inj_left a b c : c + a = c + b -> a = b.
-Proof.
-  elim: c => //; eauto.
-Qed.
-
-Lemma inj_constr_shift e e' n : e %! n == e' %! n -> e == e'.
-Proof.
-  elim: e e' n; intros until e'; case: e'; simpl; auto.
-  intro_to is_true.
-  case /eqP.
-  move /add_inj_left => ->.
-  elim: l H l0; intros until l0; case: l0; simpl; auto.
-  - move => a l; inversion.
-  - inversion.
-  - move: H0; simpl; case => H00 H01.
-    move => a0 l0; inversion.
-    apply /eqP; f_equal.
-    f_equal.
-    apply /eqP.
-    apply: H00.
-    apply /eqP; eauto.
-    suff: (con n0 l == con n0 l0); [by case /eqP|].
-    apply: H; eauto.
-Qed.
-
-Lemma inj_map_constr_shift c c' n : c::%! n == c' ::%! n -> c == c'.
-Proof using .
-  elim: c c'; intros until c'; case: c'; simpl; auto.
-  intro_to is_true.
-  case /eqP => /eqP => aeq /eqP => leq.
-  apply /eqP; f_equal; apply /eqP.
-  apply: inj_constr_shift; eauto.
-  eauto.
-Qed.
-
-Ltac solve_subpar_eq_surjective :=
-  match goal with
-      | |- ?c ::%! _ = ?c' ::%! _ => 
-        suff: c = c' => [-> //|]
-      | |- ?e %! _ = ?e'%! _ => 
-        suff: e = e' => [-> //|]
-      end;
-      apply /eqP;
-      first[ apply: inj_map_constr_shift | apply: inj_constr_shift];
-      apply /eqP;
-      repeat match goal with H : _ = _ |- _ => move: H end;
-      rewrite ?map_constr_shift_shift ?constr_shift_shift; eauto.
-
-
-Lemma first_rule_wf l a : wf_lang (a :: l) -> wf_rule (a :: l) a.
-Proof using .
-  inversion. eapply mono_rule; eauto with judgment.
-Qed.
-
-
-(*TODO: will eventually want a library of better induction schemes for same reason I wanted parameters*)
-
-(* TODO: move to utils*)
-Lemma nth_error_size_lt {A} (l : seq A) n e : List.nth_error l n = Some e -> n < size l.
-Proof.
-  elim: n l => [| n IH];case; simpl; auto; try done.
-Qed.
-
-  
-Ltac wf_to_ctx_from_rule :=
-  intro_to is_true;
-  move /rule_in_wf;
-  let H := fresh in
-  move => H;
-  match goal with
-    H : ?E, H' : ?E -> _ |- _ =>
-    specialize (H' H)
-  end;
-  inversion H.
-*)
-*)
-
-
-Lemma len_eq_size {A B} (l1 : list A) (l2 : list B) : len_eq l1 l2 -> size l1 = size l2.
-Proof using .
-  elim; intros; simpl in *; auto.
-Qed.
-
-Lemma unsubst_id s (c : ctx)
-  : all_fresh c -> len_eq s c -> s = (map var (map fst c))[/with_names_from c s/].
-Proof using .
-  elim: s c; intros until c; case: c.
-  all: repeat match goal with
-  | [|- forall _:(_*_),_] => case; intro; intro
-  | [|- forall _:seq _,_] => intro
-  | [|- is_true (all_fresh (_::_)) -> _] => simpl; move /andP; case
-  | [|- is_true (all_fresh _) -> _] => intro
-  | [|- is_true (fresh _ _) -> _] => intro
-  | [|- is_true (_ \notin _) -> _] => intro
-  | [|- is_true (all_notin (_::_)) -> _] => simpl; move /andP; case
-  | [|- is_true (all_notin _) -> _] => intro
-  | [|- len_eq _ _ -> _] => inversion; subst; try done
-  end.  
-  simpl.
-  f_equal.
-  {
-    cbn.
-    rewrite eqb_refl.
-    reflexivity.
-  }
-  {
-    simpl in H.
-    inversion H0; subst.
-    specialize (H l0 b0 H2).
-    move: H.
-    case.
-    fold_Substable.
-    rewrite ws_args_mono; eauto with judgment.
-    {
-      simpl.
-      rewrite map_fst_with_names_from; eauto with judgment.
-      auto using len_eq_size.
-    }
-    {
-      clear H0 H3 a1 b0.
-      elim: l0 l H2; intro_to (@len_eq exp (string*sort));inversion; subst;
-        intros; break; try by simpl in *; auto.
-      simpl in *.
-      rewrite in_cons eq_refl.
-      simpl.
-      auto using ws_args_ext_ctx.
-    }
-  }
-Qed.
-
-
-Lemma unsubst_id_sort n s (c : ctx)
-  : all_fresh c -> len_eq s c -> (scon n s) = (scon n (map var (map fst c)))[/with_names_from c s/].
-Proof using .
-  intros.
-  simpl.
-  f_equal.
-  by apply unsubst_id.
-Qed.
-
-Lemma unsubst_id_term n s (c : ctx)
-  : all_fresh c -> len_eq s c -> (con n s) = (con n (map var (map fst c)))[/with_names_from c s/].
-Proof using .
-  intros.
-  simpl.
-  f_equal.
-  by apply unsubst_id.
-Qed.  
-
-Lemma le_args_le_subst l c c' s1 s2
-  : le_args l c c' s1 s2 -> le_subst l c c' (with_names_from c' s1) (with_names_from c' s2).
-Proof using .
-  elim; intros; simpl in *; eauto with judgment.
-Qed.
-
-  
-(* combines le_sort_by and le_sort_subst *)
-Lemma le_sort_refl' name l c : forall c' s1 s2,
-    ws_lang l ->
-    [s| !c' |- name]%rule \in l ->
-    len_eq s1 c' ->
-    len_eq s2 c' ->
-    le_args l c c' s1 s2 ->
-    le_sort l c (scon name s1) (scon name s2).
-Proof using .
-  intros.
-  apply rule_in_ws in H0; auto.
-  simpl in *; break.
-  erewrite unsubst_id_sort; eauto.
-  replace (scon name s2) with (scon name (map var (map fst c')))[/with_names_from c' s2/];
-    [| erewrite <-unsubst_id_sort; eauto].
-  eapply le_sort_subst.
-  eapply le_args_le_subst; auto.
-  reflexivity.
-  all: eauto using ws_all_fresh_ctx, wf_is_ws_ctx.
-Qed.
-
-(* combines le_sort_by and le_sort_subst *)
-Lemma le_term_refl' name l c : forall c' s1 s2 t' t,
-    ws_lang l ->
-    [:| !c' |- name : {t'}]%rule \in l ->
-    len_eq s1 c' ->
-    len_eq s2 c' ->
-    t = t'[/with_names_from c' s2/] ->
-    le_args l c c' s1 s2 ->
-    le_term l c t (con name s1) (con name s2).
-Proof using .
-  intros.
-  repeat (match goal with [eqH : _ = _ |- _] => rewrite eqH; clear eqH end).
-  apply rule_in_ws in H0; auto; simpl in *; break.
-  inversion H0; subst.
-  erewrite unsubst_id_term; eauto.
-  replace (con name s2) with (con name (map var (map fst c')))[/with_names_from c' s2/];
-    [| erewrite <-unsubst_id_term; eauto].
-  eapply le_term_subst.
-  eapply le_args_le_subst; auto.
-  reflexivity.
-  all: eauto using ws_all_fresh_ctx, wf_is_ws_ctx.
-Qed.
-
-(* combines le_sort_by and le_sort_subst *)
-Lemma le_sort_by' name l c : forall c' e1 e2 s1 s2 e1' e2',
-    [s> !c' |- (name) {e1} = {e2} ]%rule \in l ->
-    len_eq s1 c' ->
-    len_eq s2 c' -> 
-    e1' = e1[/with_names_from c' s1/] ->
-    e2' = e2[/with_names_from c' s2/] ->
-    le_args l c c' s1 s2 ->
-    le_sort l c e1' e2'.
-Proof using .
-  intros.
-  repeat (match goal with [eqH : _ = _ |- _] => rewrite eqH; clear eqH end).
-  eapply le_sort_subst;[ | eapply le_sort_by; eassumption].
-  apply le_args_le_subst; auto.
-Qed.
-
-(* combines le_term_by and le_term_subst *)
-Lemma le_term_by' name l c : forall c' t e1 e2 s1 s2 t' e1' e2',
-    [:> !c' |- (name) {e1} = {e2} : {t}]%rule \in l ->
-    len_eq s1 c' ->
-    len_eq s2 c' ->                          
-    t' = t[/with_names_from c' s2/] ->
-    e1' = e1[/with_names_from c' s1/] ->
-    e2' = e2[/with_names_from c' s2/] ->
-    le_args l c c' s1 s2 ->
-    le_term l c t' e1' e2'.
-Proof using .
-  intros.
-  repeat (match goal with [eqH : _ = _ |- _] => rewrite eqH; clear eqH end).
-  eapply le_term_subst;[ | eapply le_term_by; eassumption].
-  apply le_args_le_subst; auto.
-Qed.
-
-Arguments le_term_by' name [l] {c} {c'} {t} {e1} {e2} {s1} {s2} {t'} {e1'} {e2'}.
-
-(* TODO: prove id-lang lemma? *)
-
-
-
-Lemma le_term_by_nameless (l : lang) c e1 e2 t
-  : term_le c e1 e2 t \in (map snd l) -> Core.le_term l c t e1 e2.
-Proof using .
-  move /in_map_snd; case;
-  intros; eapply le_term_by; eauto with judgment.
-Qed.
-
-Lemma le_sort_by_nameless (l : lang) c t1 t2
-  : sort_le c t1 t2 \in (map snd l) -> Core.le_sort l c t1 t2.
-Proof using .
-  move /in_map_snd; case;
-  intros; eapply le_sort_by; eauto with judgment.
-Qed.  
-
-
-(* TODO: Justification for eliding typing guarantees in inductive for le.
-Sufficient, but prob. not provable directly:
-Lemma le_sort_preserves_wf l c t1 t2
-  : wf_lang l -> wf_sort l c t1 -> le_sort l c t1 t2 -> wf_sort l c t2.
-Proof.
-  intros wfl wft.
-  elim.
-  {
-    
-    intros.
-*)
+  with wf_ctx_ind' := Minimality for wf_ctx Sort Prop.
+Combined Scheme judge_ind
+         from le_sort_ind', le_term_ind', le_subst_ind',
+              wf_sort_ind', wf_term_ind', wf_args_ind',
+              wf_ctx_ind'.
+
+(*TODO: separate file for properties?*)
