src/named/Elab.v
@@ -1,0 +1,75 @@
+Set Implicit Arguments.
+Set Bullet Behavior "Strict Subproofs".
+
+Require Import List String.
+Import ListNotations.
+Open Scope string.
+Open Scope list.
+From Utils Require Import Utils.
+From Named Require Import Exp ARule.
+(*TODO: why does this generate warnings?*)
+Import Exp.Notations.
+Import ARule.Notations.
+  
+Section TermsAndRules.
+  Context (l' : lang).
+
+  (* Assumes that the inputs are well-formed in the appropriate settings*)
+  Inductive elab_term : exp -> exp -> Prop :=
+  | elab_var x : elab_term (var x) (var x)
+  | elab_con n s s' c' args t
+    : In (n, (term_rule c' args t)) l' ->
+      elab_args args s (map fst c') s' ->
+      elab_term (con n s) (con n s')
+  with elab_args : list string -> list exp -> list string -> list exp -> Prop :=
+  | elab_args_nil : elab_args [] [] [] []
+  | elab_args_cons_ex e e' s s' n args args'
+    : elab_term e e' ->
+      elab_args args s args' s' ->
+      elab_args (n::args) (e::s) (n::args') (e'::s')
+  | elab_args_cons_im e e' s s' n args args'
+    : elab_term e e' ->
+      elab_args args s args' s' ->
+      elab_args args s (n::args') (e'::s').
+
+  Inductive elab_sort : sort -> sort -> Prop :=
+  | elab_scon n s s' c' args
+    : In (n, (sort_rule c' args)) l' ->
+      elab_args args s (map fst c') s' ->
+      elab_sort (scon n s) (scon n s').
+  
+  Definition elab_subst : subst -> subst -> Prop :=
+    List.Forall2 (fun '(n,t) '(n',t') => n = n' /\ elab_term t t').
+
+  Definition elab_ctx : ctx -> ctx -> Prop :=
+    List.Forall2 (fun '(n,t) '(n',t') => n = n' /\ elab_sort t t').
+
+  Variant elab_rule : rule -> rule -> Prop :=
+  | elab_sort_rule : forall c c' args,
+      elab_ctx c c' ->
+      elab_rule (sort_rule c args) (sort_rule c' args)
+  | elab_term_rule : forall c c' args t t',
+      elab_ctx c c' ->
+      elab_sort t t' ->
+      elab_rule (term_rule c args t) (term_rule c' args t')
+  | elab_le_sort_rule : forall c c' t1 t2 t1' t2',
+      elab_ctx c c' ->
+      elab_sort t1 t1' ->
+      elab_sort t2 t2' ->
+      elab_rule (sort_le c t1 t2) (sort_le c' t1' t2')
+  | elab_le_term_rule : forall c c' e1 e1' e2 e2' t t',
+      elab_ctx c c' ->
+      elab_sort t t' ->
+      elab_term e1 e1' ->
+      elab_term e2 e2' ->
+      elab_rule (term_le c e1 e2 t) (term_le c' e1' e2' t').
+End TermsAndRules.
+  
+Inductive elab_lang : lang -> lang -> Prop :=
+| elab_lang_nil : elab_lang [] []
+| elab_lang_cons n l l' r r'
+  : elab_lang l l' ->
+    elab_rule l' r r' ->
+    elab_lang ((n,r)::l) ((n,r')::l').
+
+Hint Constructors elab_lang elab_rule elab_sort List.Forall2 elab_args elab_term : exp.
